Tidying and specs

Clap/Lang/F/Tactics.lean
@@ -1,63 +1,21 @@
 import Lean
 import Clap.eDSLState.eDSL
-import Clap.eDSLState.Convert
+import Clap.eDSLState.Convert.Base
 import Clap.Lang.F.Extensions
 
-namespace Clap
 
-section
+section Helpers
 
 open Lean Elab Tactic Meta
 
-def baseNamespace := Name.mkStr2 "Clap" "Lang"
-
-def lemmaOfIdentifiers (prefixNamespace lemmaName : Name) : MetaM ConstantInfo := do
-  let name := baseNamespace ++ prefixNamespace ++ lemmaName
-  let .some «lemma» := (←getEnv).find? name
-    | throwError m!"Undeclared constant: {name}"
-  return «lemma»
-
-def convertsMargs (convertsME convertsMT : Lean.Expr) (goal : MVarId) :
-  MetaM (Option (Lean.Expr × Lean.Expr × Lean.Expr × Lean.Expr × Lean.Expr × Lean.Expr × Lean.Expr)) := goal.withContext do
-  -- logInfo m!"In"
-  let convertsMT ← instantiateMVars convertsMT
-  -- logInfo m!"Instantiated"
-  match_expr convertsMT with
-  | Clap.ConvertsM p α _ action state _ => return .some (
-      -- ←Expr.mkDirectProjection convertsMT `result,
-      ←mkAppM ``Clap.ConvertsM.result #[convertsME],
-      -- ←Expr.mkDirectProjection convertsMT `wellFormed,
-      ←mkAppM ``Clap.ConvertsM.wellFormed #[convertsME],
-      -- ←Expr.mkDirectProjection convertsMT `constraints,
-      ←mkAppM ``Clap.ConvertsM.constraints #[convertsME],
-      p,
-      α,
-      action,
-      state
-    )
-  | _ => return .none
-
-
--- def convertsLemmaAndStateOfType (convertsT : Lean.Expr) : MetaM (ConstantInfo × Lean.Expr) := do
---   let convertsT ← instantiateMVars convertsT
---   let (prefixNamespace, st) :=
---     match_expr convertsT with
---     | Clap.Lang.FList.Converts _ st _ _ => (`FList, st)
---     | Clap.Lang.FArray.Converts _ st _ _ => (`FArray, st)
---     | Clap.Lang.FUnit.Converts _ st _ _ => (`FUnit, st)
---     | Clap.Lang.FB.Converts _ st _ _ => (`FB, st)
---     | Clap.Lang.F.Converts _ st _ _ => (`F, st)
---     | _ => unreachable!
---   return (←lemmaOfIdentifiers prefixNamespace `converts_skip, st)
-
-def _root_.Lean.Meta.Hypothesis.ofNameValue (userName : Name) (value : Lean.Expr) : MetaM Hypothesis := do
+def Lean.Meta.Hypothesis.ofNameValue (userName : Name) (value : Lean.Expr) : MetaM Hypothesis := do
   return {
     userName := userName
     type     := ←inferType value
     value    := value
   }
 
-def _root_.Lean.MVarId.set (goal : MVarId) (name : Name) (rhs : Term) : MetaM MVarId := do
+def Lean.MVarId.set (goal : MVarId) (name : Name) (rhs : Term) : MetaM MVarId := do
   let ident := mkIdent name
   let ([goal], _) ← runTactic goal (←`(tactic| set $ident:ident := $rhs))
     | throwError m!"set failed (rhs := {rhs})"
@@ -66,65 +24,146 @@ def _root_.Lean.MVarId.set (goal : MVarId) (name : Name) (rhs : Term) : MetaM MV
 /--
 Execute `set`s in order, ensuring the local context is updated between every invocation.
 -/
-def _root_.Lean.MVarId.setManyInOrder (goal : MVarId) (nameXrhs : List (Name × Term)) : MetaM MVarId :=
+def Lean.MVarId.setManyInOrder (goal : MVarId) (nameXrhs : List (Name × Term)) : MetaM MVarId :=
   nameXrhs.foldlM (fun acc (name, rhs) ↦ do acc.withContext do acc.set name rhs) goal
 
+end Helpers
+
+
+namespace Clap.Tactic
+
+open Lean Elab Tactic Meta
+
+section Parsing
+
+structure ConvertsArgs where
+  p : Lean.Expr
+  α : Lean.Expr
+  conversion : Lean.Expr
+  state : Lean.Expr
+  exprs : Lean.Expr
+  val : Lean.Expr
+
+structure ConvertsMArgs where
+  p : Lean.Expr
+  α : Lean.Expr
+  conversion : Lean.Expr
+  action : Lean.Expr
+  state : Lean.Expr
+  val : Lean.Expr
+  constraints : Lean.Expr
+
+structure ConvertsMExpr where
+  args : ConvertsMArgs
+  result : Lean.Expr
+  wellFormed : Lean.Expr
+  constraints : Lean.Expr
+
+def parseConverts (convertsT : Lean.Expr) (goal : MVarId) :
+  MetaM (Option ConvertsArgs)
+:= goal.withContext do
+  let convertsT ← instantiateMVars convertsT
+  match_expr convertsT with
+  | Clap.Converts p α conversion state exprs val => return .some {
+      p := p,
+      α := α
+      conversion := conversion
+      state := state
+      exprs := exprs
+      val := val
+    }
+  | _ => return .none
+
+def parseConvertsMArgs (convertsMT : Lean.Expr) (goal : MVarId) :
+  MetaM (Option ConvertsMArgs)
+:= goal.withContext do
+  let convertsMT ← instantiateMVars convertsMT
+  match_expr convertsMT with
+  | Clap.ConvertsM p α conversion action state val constraints => return .some {
+      p,
+      α,
+      conversion,
+      action,
+      state,
+      val,
+      constraints
+    }
+  | _ => return .none
+
+def parseConvertsM (convertsME convertsMT : Lean.Expr) (goal : MVarId) :
+  MetaM (Option ConvertsMExpr)
+:= goal.withContext do
+  let convertsMT ← instantiateMVars convertsMT
+  let args ← parseConvertsMArgs convertsMT goal
+  let result ← mkAppM ``Clap.ConvertsM.result #[convertsME]
+  let wellFormed ← mkAppM ``Clap.ConvertsM.wellFormed #[convertsME]
+  let constraints ← mkAppM ``Clap.ConvertsM.constraints #[convertsME]
+  return args.map λ args => {
+    args,
+    result,
+    wellFormed,
+    constraints
+  }
+
+end Parsing
+
+
+section Tactic
+
 /--
-Yields tuples `(namespace, fvar, state, type)` of local hypotheses of the shape `<_>.Converts`.
+Yields fvars of local hypotheses of the shape `<_>.Converts`.
+Warns if they are over multiple distinct states
 -/
 def stateAssertions (goal : MVarId) :
-  MetaM (Array (Lean.Expr × Lean.Expr × Lean.Expr)) := goal.withContext do
+  MetaM (Array Lean.Expr)
+:= goal.withContext do
   let allAssertions := (←getLCtx).getFVars
   let allAssertionsT ← allAssertions.filterMapM fun fvar ↦ do
     let type ← instantiateMVars (←inferType fvar)
-    return match_expr type with
-    | Clap.Converts _ _ _ st _ _ => .some (fvar, st, type)
-    | _ => .none
-  if (allAssertionsT.groupByKey (fun (_, st, _) ↦ st) |>.size) > 1
+    let args ← parseConverts type goal
+    return args.map λ args => (fvar, args)
+  if (allAssertionsT.groupByKey (fun (_, args) ↦ args.state) |>.size) > 1
   then
     -- logWarning m!"OUR GUY:\n{(allAssertionsT.groupByKey fun (_, _, st, _) ↦ st).toArray}"
     logWarning m!"Assumptions of shape `Converts` refer to multiple states. Are you ~~mad~~ sure?"
-  return allAssertionsT
+  return allAssertionsT.map Prod.fst
 
 def lemmaOfNextCommand (goal : MVarId) : MetaM (Option Lean.Expr) := do
   let conclusion ← (instantiateMVars (←goal.getType))
-  let_expr Clap.ConvertsM _ _ _ action _ _ := conclusion |
+  let .some args ← parseConvertsMArgs conclusion goal |
     logWarning m!"Cannot infer the next step - expected `Clap.ConvertsM`.\nGot instead:\n{conclusion}"
     return .none
-  let ⟨name, _args⟩ := action.getAppFnArgs
+  let ⟨name, _args⟩ := args.action.getAppFnArgs
 
-  if name == `Bind.bind then logInfo m!"Bind.bind"; return mkConst `Clap.convertsM_bind
-  if name == `Functor.map then logInfo m!"Functor.map"; return mkConst `Clap.convertsM_map
+  if name == `Bind.bind then
+    -- logInfo m!"Bind.bind";
+    return mkConst `Clap.convertsM_bind
+  if name == `Functor.map then
+    -- logInfo m!"Functor.map";
+    return mkConst `Clap.convertsM_map
 
-  logInfo m!"Conclusion unchanged; spec missing for:\n{action}"
+  logWarning m!"Conclusion unchanged; spec missing for:\n{args.action}"
   return .none
 
 def step_impl (convertsME : Lean.Expr) (actionName : Name) (goal : MVarId) : TermElabM MVarId := goal.withContext do
-  logInfo m!"GOAL α: {goal}"
   let convertsMType ← inferType convertsME
-  logInfo m!"convetsME: {convertsME}\nconvertsMType: {convertsMType}"
-  -- logInfo m!"convertsMType : {convertsMType}"
-  -- logError m!"Expected ConvertsM. Got:\n{convertsMType}"
-  let .some (convertsConvertsM, wellFormedConvertsM, constraintsConvertsM, pE, αE, actionE, stateE) ←
-    convertsMargs convertsME convertsMType goal
+  let .some convertsM ←
+    parseConvertsM convertsME convertsMType goal
     | logError m!"Expected ConvertsM. Got:\n{convertsMType}"
       return goal
-  let stateS ← Term.exprToSyntax stateE
-  let stepE := convertsConvertsM
-  let hypWFE := wellFormedConvertsM
-  let hypConstraintsE := constraintsConvertsM
+  let stateS ← Term.exprToSyntax convertsM.args.state
   let stateAssertions ← stateAssertions goal
-  let assertions ← stateAssertions.mapM fun (fvar, state, type) ↦ do
+  let assertions ← stateAssertions.mapM fun fvar ↦ do
     return (fvar, ←mkAppM `Clap.converts_skip #[convertsME, fvar])
   let goal ← assertions.foldlM (init := goal) fun goal (fvar, _) ↦
     goal.clear fvar.fvarId!
 
   let (_, goal) ← goal.assertHypotheses <|
     #[
-      ←Hypothesis.ofNameValue (actionName.appendBefore "h_") stepE,
-      ←Hypothesis.ofNameValue `h_wellFormed hypWFE,
-      ←Hypothesis.ofNameValue `h_constraints hypConstraintsE,
-    ] 
+      ←Hypothesis.ofNameValue (actionName.appendBefore "h_") convertsM.result,
+      ←Hypothesis.ofNameValue `h_wellFormed convertsM.wellFormed,
+      ←Hypothesis.ofNameValue `h_constraints convertsM.constraints,
+    ]
     ++ (
       ←assertions.mapM fun (fvar, expr) ↦ do
         let name := ((←getLCtx).get! fvar.fvarId!).userName
@@ -138,7 +177,7 @@ def step_impl (convertsME : Lean.Expr) (actionName : Name) (goal : MVarId) : Ter
 
   goal.setManyInOrder [
     -- `set action := <action_from_monad>`
-    (actionName, ←Term.exprToSyntax actionE),
+    (actionName, ←Term.exprToSyntax convertsM.args.action),
     -- `set <action>_result := <action>.getResult <state>.numAlloc <state>.σ`
     (actionName.appendAfter "_result", ←`($(actionIdent).getResult $(stateS).numAlloc $(stateS).σ)),
     -- `set <state> := <action>.getState <state>`
@@ -148,7 +187,7 @@ def step_impl (convertsME : Lean.Expr) (actionName : Name) (goal : MVarId) : Ter
 elab "step" convertsM:term "as" actionName:ident : tactic => withMainContext do
   let goal ← getMainGoal
   let convertsME ← instantiateMVars (←elabTerm convertsM .none)
-  discard do 
+  discard do
     match ←lemmaOfNextCommand goal with
     | .none => pure ()
     | .some stepConclusion =>
@@ -158,49 +197,55 @@ elab "step" convertsM:term "as" actionName:ident : tactic => withMainContext do
   let goal ← step_impl convertsME actionName.getId (←getMainGoal)
   replaceMainGoal [goal]
 
-elab "finish" : tactic => withMainContext do
-  let target ← whnf (←getMainTarget)
+-- Used for if step is missing functionality for the specific shape of conclusion
+elab "step_state" convertsM:term "as" actionName:ident : tactic => withMainContext do
+  let convertsME ← instantiateMVars (←elabTerm convertsM .none)
+  let goal ← step_impl convertsME actionName.getId (←getMainGoal)
+  replaceMainGoal [goal]
 
-  if !target.isAppOf ``Clap.ConvertsM
-  then logWarning m!"Made no progress - the concluson must be of shape ConvertsM."
-       return ()
+-- elab "finish" : tactic => withMainContext do
+--   let target ← whnf (←getMainTarget)
 
-  let result :: goalsRest ← (←getMainGoal).constructor | unreachable!
-  for goal in goalsRest do
-    try
-      let ([], _) ← runTactic goal (←`(tactic| grind)) | continue
-    catch _ =>
-      continue
-  
-  let goalsRest ← goalsRest.filterM fun goal ↦ return !(←goal.isAssigned)
+--   if !target.isAppOf ``Clap.ConvertsM
+--   then logWarning m!"Made no progress - the concluson must be of shape ConvertsM."
+--        return ()
 
-  let lastConvertsM := stepExt.getState (← getEnv) |>.lastLemmaUserName
-  let lastConvertsME := (←getLCtx).getFromUserName! lastConvertsM |>.toExpr
-  
-  let conclusionT ← result.getType'
-  let_expr Clap.Converts _ _ _ st _ _ := conclusionT |
-    throwError m!"Finish expects Clap.ConvertsM - failed to extract converts. Bad."
+--   let result :: goalsRest ← (←getMainGoal).constructor | unreachable!
+--   for goal in goalsRest do
+--     try
+--       let ([], _) ← runTactic goal (←`(tactic| grind)) | continue
+--     catch _ =>
+--       continue
 
-  let lastConvertsMT ← instantiateMVars (←inferType lastConvertsME)
-  let_expr Clap.Converts _ _ _ st' _ _ := lastConvertsMT |
-    throwError m!"Could not extract Clap.Converts from the previous step command. Bad."
+--   let goalsRest ← goalsRest.filterM fun goal ↦ return !(←goal.isAssigned)
 
-  logInfo m!"st: {st}\nst': {st'}"
+--   let lastConvertsM := stepExt.getState (← getEnv) |>.lastLemmaUserName
+--   let lastConvertsME := (←getLCtx).getFromUserName! lastConvertsM |>.toExpr
 
-  -- if !(←isDefEq st st')
-  -- then throwError m!"State does not match the state from the previous step. Bad."
+--   let conclusionT ← result.getType'
+--   let_expr Clap.Converts _ _ _ st _ _ := conclusionT |
+--     throwError m!"Finish expects Clap.ConvertsM - failed to extract converts. Bad."
 
-  let ([result], _) ←
-    try
-      runTactic result
-        (←`(tactic| apply Clap.converts_of_converts $(←Term.exprToSyntax lastConvertsME)))
-    catch _ =>
-      return default
-    | logWarning m!"Cannot apply Clap.converts_of_converts"
+--   let lastConvertsMT ← instantiateMVars (←inferType lastConvertsME)
+--   let_expr Clap.Converts _ _ _ st' _ _ := lastConvertsMT |
+--     throwError m!"Could not extract Clap.Converts from the previous step command. Bad."
 
-  let (goals, _) ← runTactic result (←`(tactic| try with_reducible rfl))
-  replaceMainGoal (goals ++ goalsRest)
+--   logInfo m!"st: {st}\nst': {st'}"
 
-end
+--   -- if !(←isDefEq st st')
+--   -- then throwError m!"State does not match the state from the previous step. Bad."
 
-end Clap
+--   let ([result], _) ←
+--     try
+--       runTactic result
+--         (←`(tactic| apply Clap.converts_of_converts $(←Term.exprToSyntax lastConvertsME)))
+--     catch _ =>
+--       return default
+--     | logWarning m!"Cannot apply Clap.converts_of_converts"
+
+--   let (goals, _) ← runTactic result (←`(tactic| try with_reducible rfl))
+--   replaceMainGoal (goals ++ goalsRest)
+
+end Tactic
+
+end Clap.Tactic
