Clap/Lang/FB/and.lean
@@ -1,67 +1,32 @@
-import Clap.Lang.FB.FB
+import Clap.Lang.F.mkMul
 
-namespace Clap.Edsl.Lang.FB
+namespace Clap.Lang.FB
 
-section
+variable {p : ℕ}
 
-variable {p : ℕ} [p.AtLeastTwo] {varStore : VarStore p} {x y : FB p}
-
-def and (a b : FB p) : FB p := a * b
+def and (a b : FB) : ClapM p FB := do
+  HashConsM.mkMul (p := p) a b
 
 namespace and
 
-@[grind .]
-lemma and_false (x_valid : x.isValid varStore) (y_valid : y.isValid varStore) :
-  [varStore|x.and y] = [varStore|FB.false p] ↔
-  [varStore|x] = [varStore|FB.false p] ∨ [varStore|y] = [varStore|FB.false p]
+lemma convertsM
+  [p.AtLeastTwo]
+  {state : ClapMState p}
+  {a b : FB}
+  {a_val b_val : Bool}
+  (h_a : Converts FB.conversion state a a_val)
+  (h_b : Converts FB.conversion state b b_val)
+:
+  ConvertsM FB.conversion (and a b) state (a_val && b_val) True
 := by
-  simp [FB.and, FixedExp.mul_def, eval_false]
-  constructor
-  · rcases [varStore|x] <;> rcases _ : [varStore|y] <;> grind
-  · rintro (h₁ | h₂) <;> rcases _ : [varStore|x] <;> grind
+  unfold and
+  have h_a_f := F.converts_of_FB_converts h_a
+  have h_b_f := F.converts_of_FB_converts h_b
+  have h_mul := mkMul.convertsM h_a_f h_b_f
+  have h_mul_FB := FB.convertsM_of_F_convertsM h_mul
+  apply convertsM_of_convertsM (h_mul_FB _)
+  . grind
+  . trivial
+  . cases a_val <;> cases b_val <;> simp
 
-@[grind .]
-lemma and_true :
-  ([varStore|x] = [varStore|FB.true p]) ∧ ([varStore|y] = [varStore|FB.true p])
-  ↔
-  (x.isValid varStore ∧ y.isValid varStore ∧ [varStore|x.and y] = [varStore|FB.true p])
-:= by
-  simp [FB.and, FixedExp.mul_def, eval_true]
-  rcases _ : [varStore|y] <;> rcases _ : [varStore|x] <;> grind
-
-@[grind .]
-lemma and_ofBool {b₁ b₂ : Bool}
-  (h: [varStore|x] = [varStore|FB.ofBool p b₁])
-  (h: [varStore|y] = [varStore|FB.ofBool p b₂]) :
-  [varStore|x.and y] = [varStore|FB.ofBool p (b₁ && b₂)]
-:= by
-  grind
-
-@[grind .]
-lemma toIdeal_and {a b : FB p} {a' b' : Bool}
-  (h₁ : Convert.toIdeal varStore a = .some a')
-  (h₂ : Convert.toIdeal varStore b = .some b') :
-  Convert.toIdeal varStore (a.and b) = .some (a' && b')
-:= by
-  have valid₁ := (Convert.isValid_iff_isSome_toIdeal varStore a).mpr (by
-    rw! [h₁]; rfl
-  )
-  have valid₂ := (Convert.isValid_iff_isSome_toIdeal varStore b).mpr (by
-    rw! [h₂]; rfl
-  )
-  rewrite [toIdeal_def] at h₁ h₂ ⊢
-  unfold toBool at h₁ h₂ ⊢
-  simp_all only [beq_iff_eq, isValid_iff]
-  cases valid₁ <;> grind
-
-lemma equiv :
-  matchesBinaryFunction p (· && ·) (FB.and (p := p))
-:= by
-  unfold matchesBinaryFunction
-  grind
-
-end and
-
-end
-
-end Clap.Edsl.Lang.FB
+end Clap.Lang.FB.and
