Clap/Lang/FB/assert.lean
@@ -1,179 +1,30 @@
-import Clap.Lang.FB.FB
 import Clap.Lang.FB.not
+import Clap.Lang.FUnit.eq0
 
-namespace Clap.Edsl.Lang.FB
+namespace Clap.Lang
 
-def assert {p : ℕ} [p.AtLeastTwo] (a : FB p) : Edsl.CircuitM p Unit := do
-  Edsl.eq0 (not a)
+variable {p : ℕ}
+
+def assert (a : FB) : ClapM p Unit := do
+  eq0 (←not a)
 
 namespace assert
 
-@[simp, grind .]
-lemma isAlwaysValid_unit
-  {p : ℕ}
+lemma convertsM
   [p.AtLeastTwo]
-  {numAlloc : ℕ}
-  {varStore : VarStore p}
-  {f : Edsl.CircuitM p Unit}
+  {state : ClapMState p}
+  {a : FB}
+  {a_val : Bool}
+  (h_a : Converts FB.conversion state a a_val)
 :
-  IsValid.isValid varStore (f.getResult numAlloc)
-:= by
-  trivial
-
-@[simp, grind =]
-lemma toIdeal_unit
-  {p : ℕ}
-  {varStore : VarStore p}
-  {x : Unit}
-:
-  Convert.toIdeal varStore x = .some ()
-:= by
-  trivial
-
-@[simp, grind =]
-lemma getResult_unit
-  {p : ℕ}
-  {numAlloc : ℕ}
-  {f : Edsl.CircuitM p Unit}
-:
-  f.getResult numAlloc = ()
-:= rfl
-
-@[grind =]
-lemma step_eq0_fb
-  {p : ℕ}
-  [p.AtLeastTwo]
-  {a : FB p}
-  {result : CircuitResult p}
-:
-  [result|Gate.eq0 a]ₛ =
-  result.addConstraint ([result.varStore|a] = [result.varStore|false p])
-:= rfl
-
-@[grind =]
-lemma assert_constraints
-  {p : ℕ}
-  [p.AtLeastTwo]
-  {varStore : VarStore p}
-  {a : FB p}
-  {numAlloc : ℕ}
-  (h: IsValid.isValid varStore a)
-:
-  [varStore, numAlloc|(a.assert.getCircuit numAlloc)]ₑ.constraints =
-  ((Convert.toIdeal varStore a).get (by grind) = Bool.true)
+  ConvertsM FUnit.conversion (assert a) state () (a_val = true)
 := by
   unfold assert
-  grind
+  step not.convertsM h_a as not
+  have h_not_f := F.converts_of_FB_converts h_not
+  apply convertsM_of_convertsM (eq0.convertsM h_not_f)
+  . rfl
+  . grind
+  . exact λ _ => True.intro
 
-@[grind =]
-lemma assert_numAlloc
-  {p : ℕ}
-  [p.AtLeastTwo]
-  {varStore : VarStore p}
-  {a : FB p}
-  {numAlloc : ℕ}
-:
-  [varStore, numAlloc|(a.assert.getCircuit numAlloc)]ₑ.numAlloc =
-  numAlloc
-:= by
-  unfold assert
-  grind
-
-@[grind =]
-lemma assert_frameRule
-  {p : ℕ}
-  [p.AtLeastTwo]
-  {varStore : VarStore p}
-  {a : FB p}
-  {numAlloc : ℕ}
-:
-  ∀ n, n < numAlloc →
-    [varStore, numAlloc|(a.assert.getCircuit numAlloc)]ₑ.varStore[n]? =
-    varStore[n]?
-:= by
-  intro n h_n
-  unfold assert
-  grind
-
-@[simp, grind =]
-lemma toLinear_unit
-  {p : ℕ}
-  [p.AtLeastTwo]
-  {varStore : VarStore p}
-:
-  VarStoreSize.toLinear varStore () =
-  #v[]
-:= by
-  rfl
-
-@[simp, grind .]
-lemma assertMatchesLast_empty
-  {p : ℕ}
-  [p.AtLeastTwo]
-  {varStore : VarStore p}
-  {numAlloc : ℕ}
-:
-  assertMatchesLast
-    varStore
-    numAlloc
-    #v[]
-:= by
-  unfold assertMatchesLast
-  grind
-
-@[simp, grind .]
-lemma assertMatchesLast_toLinear_unit
-  {p : ℕ}
-  [p.AtLeastTwo]
-  {varStore1 varStore2 : VarStore p}
-  {numAlloc : ℕ}
-  {x : Unit}
-:
-  assertMatchesLast
-    varStore1
-    numAlloc
-    (VarStoreSize.toLinear varStore2 x)
-:= by
-  unfold assertMatchesLast
-  grind
-
-@[grind .]
-lemma result_IsValid_iff
-  {p : ℕ}
-  [p.AtLeastTwo]
-  {numAlloc : ℕ}
-:
-  unaryFunctionResultIsValidIff p (λ x => (FB.assert (p := p) x).getResult numAlloc)
-:= by
-  unfold unaryFunctionResultIsValidIff assert
-  have (a : FB p) (varStorePre : VarStore p) : IsValid.isValid varStorePre ((eq0 (not a)).run numAlloc).1.1 := by
-    grind
-  grind
-
-@[grind .]
-lemma result_correct
-:
-  unaryFunctionResultIsCorrect p (!·) (FB.not (p := p))
-:= by
-  unfold unaryFunctionResultIsCorrect
-  grind [FB.toRepresents_def]
-
-lemma equiv (p : ℕ) [p.AtLeastTwo] :
-  matchesUnaryMonadFunction p
-    (spec_function := λ _ => ())
-    (function := FB.assert)
-    (allocatesN := 0)
-    (constraints := λ input => input = Bool.true)
-:= by
-  intro a varStore numAlloc h_isValid
-  have : (a.assert.runAndEval numAlloc varStore) =
-    ⟨
-      (a.assert.getResult numAlloc),
-      [varStore, numAlloc|a.assert.getCircuit numAlloc]ₑ
-    ⟩
-  := by rfl
-  grind
-
-end assert
-
-end Clap.Edsl.Lang.FB
+end Clap.Lang.assert
