Clap/Lang/FB/not.lean
@@ -1,106 +1,33 @@
-import Clap.Lang.FB.FB
+import Clap.Lang.F.mkF
+import Clap.Lang.F.mkSub
 
-namespace Clap.Edsl.Lang.FB
+namespace Clap.Lang
 
-section
+variable {p : ℕ}
 
-variable {p : ℕ} [p.AtLeastTwo] {varStore : VarStore p} {x : FB p}
-
-def not {p : ℕ} [p.AtLeastTwo] (a : FB p) : FB p := 1 - a
-
-@[simp, grind =]
-lemma bind_true {α} {varStore : VarStore p} {f : ZMod p → Option α} :
-  [varStore|true p].bind f = f ([varStore|true p].get (by grind))
-:= by
-  aesop (add simp [Option.bind, FB.true])
-
-@[simp, grind =]
-lemma bind_false {α} {varStore : VarStore p} {f : ZMod p → Option α} :
-  [varStore|false p].bind f = f ([varStore|false p].get (by grind))
-:= by
-  aesop (add simp [Option.bind, FB.false])
-
-@[grind .]
-lemma not_true:
-  ([varStore|x =Γ FB.true p]) ↔
-  ([varStore|x.not =Γ FB.false p])
-:= by
-  simp [FB.not, FixedExp.sub_def, eval_false, eval_true]
-  obtain _ | x := [varStore|x] <;> grind
-
-@[grind .]
-lemma not_false
-:
-  ([varStore|x =Γ FB.false p]) ↔
-  ([varStore|x.not =Γ FB.true p])
-:= by
-  simp [FB.not, FixedExp.sub_def, eval_false, eval_true]
-  obtain _ | x := [varStore|x] <;> grind
-
-@[grind .]
-lemma not_none
-  (h : [varStore|x] = .none)
-:
-  [varStore|x.not] = .none
-:= by
-  grind [FB.not]
-
-lemma not_ofBool {b : Bool} (h: [varStore|x] = [varStore|FB.ofBool p b]) :
-  [varStore|x.not] = [varStore|FB.ofBool p !b]
-:= by
-  grind
-
-@[grind .]
-lemma toIdeal_not {a : FB p} {b : Bool}
-  (h : Convert.toIdeal varStore a = .some b)
-:
-  Convert.toIdeal varStore a.not =
-  .some !b
-:= by
-  have := (Convert.isValid_iff_isSome_toIdeal varStore a).mpr (by
-    rw! [h]
-    rfl
-  )
-  rewrite [toIdeal_def] at h ⊢
-  unfold toBool at h ⊢
-  grind [isValid_iff]
+def not (a : FB) : ClapM p FB := do
+  let one ← mkF 1
+  mkSub one a
 
 namespace not
 
-@[aesop simp, grind .]
-lemma isValid_not_iff :
-  IsValid.isValid varStore (not x) ↔ IsValid.isValid varStore x
+lemma convertsM
+  [p.AtLeastTwo]
+  {state : ClapMState p}
+  {a : FB}
+  {a_val : Bool}
+  (h_a : Converts FB.conversion state a a_val)
+:
+  ConvertsM FB.conversion (not a) state (!a_val) True
 := by
   unfold not
-  refine Iff.intro (fun h ↦ ?p₁) (fun h ↦ ?p₂) <;>
-  aesop (add simp [FB.isValid_iff, Option.bind, FixedExp.sub_def])
+  step mkF.convertsM as one
+  have h_a_f := F.converts_of_FB_converts h_a
+  have h_sub := FB.convertsM_of_F_convertsM (mkSub.convertsM h_one h_a_f)
+  apply convertsM_of_convertsM (h_sub _)
+  . grind
+  . trivial
+  . cases a_val <;> simp
+  . trivial
 
-@[grind .]
-lemma result_IsValid_iff
-:
-  unaryFunctionResultIsValidIff p (FB.not (p := p))
-:= by
-  unfold unaryFunctionResultIsValidIff
-  grind
-
-@[grind .]
-lemma result_correct
-:
-  unaryFunctionResultIsCorrect p (!·) (FB.not (p := p))
-:= by
-  unfold unaryFunctionResultIsCorrect
-  grind [FB.toRepresents_def]
-
-@[grind .]
-lemma equiv :
-  matchesUnaryFunction p Bool.not (FB.not (p := p))
-:= by
-  grind
-
--- #spec Bool.not FB.not
-
-end not
-
-end
-
-end Clap.Edsl.Lang.FB
+end Clap.Lang.not
