Clap/Lang/F/mkF.lean
@@ -1,0 +1,39 @@
+import Clap.eDSLState.Convert.Specialised
+
+namespace Clap.Lang
+
+variable {p : ℕ}
+
+def mkF (a : ZMod p) : ClapM p F :=
+  HashConsM.mkConstant (p := p) a
+
+namespace mkF
+
+@[simp]
+lemma hashConsM_convertsM
+  {state}
+  {x : ZMod p}
+:
+  ConvertsM F.conversion (liftM (HashConsM.mkConstant (p := p) x)) state x True
+:= by
+  constructor
+  · simp [ClapM.getState]
+    simp_rw [HashConsM.getResult_mkConstant, HashConsM.getHashConsState_mkConstant]
+    constructor <;> simp
+    · grind [=Expr.varSet, =Expr.varSet_wellFormed]
+    · grind
+    · rw [eval_eq_evalRec (by grind)]
+      grind
+  · grind
+  . grind [ClapM.runAndEval]
+
+lemma convertsM
+  {state : ClapMState p}
+  {a : ZMod p}
+:
+  ConvertsM F.conversion (mkF a) state a True
+:= hashConsM_convertsM
+
+end mkF
+
+end Clap.Lang
