Clap/Lang/F/mkSub.lean
@@ -1,0 +1,50 @@
+import Clap.eDSLState.Convert.Specialised
+
+namespace Clap.Lang
+
+variable {p : ℕ}
+
+def mkSub (a b : F) : ClapM p F :=
+  HashConsM.mkSub (p := p) a b
+
+namespace mkSub
+
+lemma hashConsM_converts
+   {state}
+   {a b : ExprRef}
+   {a_val b_val : ZMod p}
+   (h_a : Converts F.conversion state a a_val)
+   (h_b : Converts F.conversion state b b_val)
+:
+  Converts F.conversion
+    (ClapM.getState (liftM (HashConsM.mkSub (p := p) a b)) state)
+    (ClapM.getResult (liftM (HashConsM.mkSub (p := p) a b)) state.numAlloc state.σ)
+    (a_val - b_val)
+:= by
+  simp [ClapM.getState]
+  obtain ⟨a_length, a_varSet, a_wellFormed, a_result⟩ := h_a
+  obtain ⟨b_length, b_varSet, b_wellFormed, b_result⟩ := h_b
+  constructor <;>
+  simp at *
+  . grind [=Expr.varSet_wellFormed]
+  . grind
+  . grind
+
+lemma convertsM
+  {state : ClapMState p}
+  {a b : F}
+  {a_val b_val : ZMod p}
+  (h_a : Converts F.conversion state a a_val)
+  (h_b : Converts F.conversion state b b_val)
+:
+  ConvertsM F.conversion (mkSub a b) state (a_val - b_val) True
+:= by
+  unfold mkSub
+  constructor
+  . exact hashConsM_converts h_a h_b
+  . grind
+  . grind [ClapM.runAndEval]
+
+end mkSub
+
+end Clap.Lang
