Clap/Lang/FArray/singleOneArray.lean
@@ -1,0 +1,96 @@
+import Clap.Lang.FArray.OneHotRaw
+import Clap.Lang.FArray.sum
+import Clap.Lang.FUnit.assert_eq
+import Clap.Lang.F.mkF
+
+namespace Clap.Lang
+
+variable {p : ℕ}
+
+section singleOneArray
+
+/-- Returns a one-hot bit mask of length `len` with a 1 at index `idx` and 0s elsewhere. Only satisfiable when `0 ≤ idx < len`. -/
+def singleOneArray [p.AtLeastTwo] (len : ℕ) (idx : F) : ClapM p (FArray len) := do
+  let out ← oneHotRaw len idx
+  let s : F ← out.sum
+  assert_eq s (←mkF 1)
+  return out
+
+namespace singleOneArray
+
+lemma Vector.sum_ofFn_eq_zero_of_eq_zero
+  {k}
+  {f : Fin k → ZMod p}
+  (h : ∀ x : Fin k, f x = 0)
+:
+  (Vector.ofFn f).sum = 0
+:= by
+  rw [
+    ←Vector.sum_toList,
+    Vector.toList_ofFn,
+    List.sum_eq_zero
+  ]
+  grind
+
+lemma convertsM
+  [p.AtLeastTwo]
+  {len : ℕ}
+  {idx : F}
+  {state}
+  {idx_val : ZMod p}
+  (h_idx : Converts F.conversion state idx idx_val)
+  (h_len : len < p)
+:
+  ConvertsM FArray.conversion (singleOneArray len idx) state (Vector.ofFn (λ x => x.val == idx_val.val)) (idx_val.val < len)
+:= by
+  unfold singleOneArray
+
+  step oneHotRaw.convertsM h_idx h_len as oneHot
+  step FArray.sum.convertsM h_oneHot as sum
+  step mkF.convertsM as one
+  step assert_eq.convertsM h_sum h_one as assert_eq
+  apply convertsM_pure
+  . exact h_oneHot
+  . simp
+    intro h_sum
+    by_contra h_idx_val
+    rewrite [Vector.sum_ofFn_eq_zero_of_eq_zero] at h_sum
+    . simp at h_sum
+    . grind
+  . simp
+    intro h_idx_val
+    clear *-h_len h_idx_val
+    induction' len with len ih
+    . grind
+    . specialize ih (by grind)
+      rewrite [Vector.ofFn_succ]
+      by_cases h: idx_val.val = len
+      . simp [h]
+        clear ih
+        have (i : Fin len) : (i.val = len) = false := by grind
+        simp [this]
+        clear *-len
+        unfold Vector.ofFn
+        simp
+        induction' len with len ih'
+        . set x := Array.ofFn _
+          have : x = #[] := rfl
+          grind
+        . rewrite [Array.ofFn_succ]
+          grind
+      . specialize ih (by grind)
+        simp
+        rewrite [ite_cond_eq_false]
+        . simp
+          convert ih
+          grind
+        . grind
+  . exact λ _ ↦ True.intro
+  . exact λ _ ↦ True.intro
+  . exact λ _ ↦ True.intro
+
+end singleOneArray
+
+end singleOneArray
+
+end Clap.Lang
