Clap/Lang/FArray/sum.lean
@@ -1,0 +1,100 @@
+import Clap.Lang.F.mkAdd
+import Clap.Lang.F.mkF
+
+namespace Clap.Lang
+
+variable {p : ℕ}
+
+section sum
+
+open HashConsM in
+def FArray.sum' {k} (init : F) (vals : FArray k) : ClapM p F := do
+  vals.foldlM mkAdd init
+
+namespace FArray.sum'
+
+lemma convertsM
+  {k}
+  {state : ClapMState p}
+  {f_vals : FArray k}
+  {vals : Vector Bool k}
+  {init : F}
+  (h_vals : Converts FArray.conversion state f_vals vals)
+  (h_init : Converts F.conversion state init 0)
+:
+  ConvertsM F.conversion (f_vals.sum' init) state (vals.map (λ x => if x then (1: ZMod p) else 0)).sum True
+:= by
+  unfold sum'
+
+  induction' k with k h_k
+  . have (init : ExprRef) : Vector.foldlM (m := ClapM p) mkAdd init f_vals = pure init := by
+      convert Vector.foldlM_empty
+      obtain ⟨⟨_⟩, _⟩ := f_vals
+      grind
+    simp [this]
+
+    apply convertsM_pure <;> [skip; exact True.intro]
+
+    have : vals = #v[] := by grind
+    simp [this]
+    assumption
+  . have := (FArray.converts_vector_cast (k2 := k) (FArray.converts_pop h_vals) (by trivial))
+    set fvals_base := Vector.cast (m := k) (by trivial) f_vals.pop
+    set vals_base := Vector.cast (m := k) (by trivial) vals.pop
+
+    have h_push : f_vals = fvals_base.push f_vals[k] := by
+      ext
+      rewrite [Vector.getElem_push]
+      split
+      . simp [fvals_base]
+      . grind
+    rewrite [h_push]
+    simp [Vector.foldlM_push]
+
+    step @h_k fvals_base vals_base this as mapM <;> [skip; trivial]
+
+    have h_fvals_k := F.converts_of_FB_converts (FArray.converts_getElem h_vals (Nat.lt_succ_self k))
+    apply convertsM_of_convertsM (mkAdd.convertsM h_mapM h_fvals_k)
+    . have : vals = vals_base.push vals[k] := by
+        ext
+        rewrite [Vector.getElem_push]
+        split
+        . simp [vals_base]
+        . grind
+      rewrite [this]
+      simp
+    . trivial
+
+
+end FArray.sum'
+
+
+
+open HashConsM in
+def FArray.sum {k} (vals : FArray k) : ClapM p F := do
+  vals.foldlM mkAdd (←mkF 0)
+
+namespace FArray.sum
+
+lemma convertsM
+  {k}
+  {state : ClapMState p}
+  {f_vals : FArray k}
+  {vals : Vector Bool k}
+  (h_vals : Converts FArray.conversion state f_vals vals)
+:
+  ConvertsM F.conversion (f_vals.sum) state (vals.map (λ x => if x then (1: ZMod p) else 0)).sum True
+:= by
+  unfold sum
+  simp [←sum'.eq_def]
+
+  step mkF.convertsM as zero <;> [skip; trivial]
+
+  apply convertsM_of_convertsM (sum'.convertsM h_vals h_zero)
+  . rfl
+  . trivial
+
+end FArray.sum
+end sum
+
+end Clap.Lang
