Clap/Lang/FB/eq.lean
@@ -1,0 +1,35 @@
+import Clap.Lang.F.mkSub
+import Clap.Lang.FB.isZero
+
+namespace Clap.Lang
+
+variable {p : ℕ}
+
+section eq
+
+def eq {p : ℕ} [p.AtLeastTwo] (a b : F) : ClapM p FB := do
+  isZero (←HashConsM.mkSub (p := p) a b)
+
+namespace eq
+
+lemma convertsM
+  [p.AtLeastTwo]
+  {state}
+  {a b : F}
+  {a_val b_val : ZMod p}
+  (h_a : Converts F.conversion state a a_val)
+  (h_b : Converts F.conversion state b b_val)
+:
+  ConvertsM FB.conversion (eq a b) state (a_val == b_val) True
+:= by
+  unfold eq
+
+  step mkSub.convertsM h_a h_b as sub <;> [skip; exact λ _ ↦ True.intro]
+  apply convertsM_of_convertsM (isZero.convertsM h_sub)
+  . grind
+  . grind
+
+end eq
+end eq
+
+end Clap.Lang
