Clap/Lang/FB/isZero.lean
@@ -1,0 +1,103 @@
+import Clap.eDSLState.Convert.Specialised
+
+namespace Clap.Lang
+
+variable {p : ℕ}
+
+namespace isZero
+
+@[simp, grind! .]
+lemma lt_getNumAlloc
+  {numAlloc : ℕ}
+  {σ : HashConsSt p}
+  {a : ExprRef}
+:
+  numAlloc < (isZero a).getNumAlloc numAlloc σ
+:= by
+  simp [isZero]
+
+lemma wellFormed {e! : ExprRef} {state} {value : ZMod p}
+  (h : Converts F.conversion state e! value)
+:
+  (isZero e!).wellFormed state.numAlloc state.varStore state.σ
+:= by
+  obtain ⟨h_varSet, h_wellFormed, h_result⟩ := h
+  simp at *
+  apply wellFormed_isZero
+  . grind
+  . have : [state.varStore|⦃e!, state.σ⦄].isSome = true := by grind
+    grind
+  . grind
+
+lemma converts
+  [p.AtLeastTwo]
+  {state}
+  {a : F}
+  {a_val : ZMod p}
+  (h_a : Converts F.conversion state a a_val)
+:
+  Converts FB.conversion
+    ((isZero a).getState state)
+    ((isZero a).getResult state.numAlloc state.σ)
+    (a_val == 0)
+:= by
+  obtain ⟨a_length, a_varSet, a_wellFormed, a_result⟩ := h_a
+  obtain ⟨varStore, σ, numAlloc⟩ := state
+  simp [ClapM.getState]
+  constructor <;> simp at *
+  . intro i h_i
+    grind [=isZero, ClapM.getState]
+  . simp [isZero]
+    rw [Expr.wellFormed_iff_isSome, Expr.deref_mkVar_eq_some]
+    rfl
+  . simp [isZero, HashConsM.mkVar]
+    simp [HashConsM.getHashConsState_saveExpr_of_wellFormed,
+          HashConsM.getResult_saveExpr_of_wellFormed]
+    split
+    · rw [eval_eq_evalRec (by grind)]
+      unfold Expr.evalRec
+      grind
+    · rw [eval_eq_evalRec (by grind)]
+      rw [evalRec_eq_of_deref_eq_some_v (idx := numAlloc)]
+      · simp
+        rw [eval_eq_evalRec (by grind)] at a_result ⊢
+        rw [←evalRec_of_wellFormed_of_prefix] at ⊢
+        · rw [a_result]
+          grind
+        · grind
+        · grind
+      · grind
+
+lemma constraints
+  {state : ClapMState p}
+  {a}
+  {a_val}
+  (h_a : Converts F.conversion state a a_val)
+:
+  ((isZero a).runAndEval state.numAlloc state.varStore state.σ).2.constraints
+:= by
+  simp
+  have : [state.varStore|⦃a, state.σ⦄].isSome := by grind
+  exact isSome_eval_of_prefix (by {
+    grind [cases Converts]
+  }) this (by rfl) (by grind)
+
+lemma convertsM
+  [p.AtLeastTwo]
+  {state}
+  {a : F}
+  {a_val : ZMod p}
+  (h_a : Converts F.conversion state a a_val)
+:
+  ConvertsM FB.conversion (isZero a)
+    state
+    (a_val == 0)
+    True
+where
+  result := converts h_a
+  wellFormed := wellFormed h_a
+  constraints := iff_true_intro (constraints h_a)
+
+end isZero
+
+end Clap.Lang
