Clap/Lang/FUnit/assert_eq.lean
@@ -1,0 +1,36 @@
+import Clap.Lang.F.mkSub
+import Clap.Lang.FUnit.eq0
+
+namespace Clap.Lang
+
+variable {p : ℕ}
+
+section assert_eq
+
+def assert_eq (a b : F) : ClapM p Unit := do
+  let diff ← HashConsM.mkSub (p := p) a b
+  eq0 diff
+
+namespace assert_eq
+
+lemma convertsM
+  [p.AtLeastTwo]
+  {a b} {a_val b_val}
+  {state : ClapMState p}
+  (h_a : Converts F.conversion state a a_val)
+  (h_b : Converts F.conversion state b b_val)
+:
+  ConvertsM FUnit.conversion (assert_eq a b) state () (a_val = b_val)
+:= by
+  unfold assert_eq
+
+  step mkSub.convertsM h_a h_b as sub <;> [skip; exact λ _ ↦ True.intro]
+
+  apply convertsM_of_convertsM (eq0.convertsM h_sub)
+  . rfl
+  . grind
+
+end assert_eq
+end assert_eq
+
+end Clap.Lang
