Clap/Lang/FUnit/eq0.lean
@@ -1,0 +1,66 @@
+import Clap.eDSLState.Convert.Specialised
+
+namespace Clap.Lang
+
+variable {p : ℕ}
+
+namespace eq0
+
+lemma wellFormed {e! : ExprRef} {state} {value : ZMod p}
+  (h : Converts F.conversion state e! value)
+:
+  (eq0 e!).wellFormed state.numAlloc state.varStore state.σ
+:= by
+  obtain ⟨h_varSet, h_wellFormed, h_result⟩ := h
+  simp at *
+  apply wellFormed_eq0
+  . grind
+  . have : [state.varStore|⦃e!, state.σ⦄].isSome = true := by grind
+    grind
+  . grind
+
+lemma converts
+  [p.AtLeastTwo]
+  {state : ClapMState p}
+  {a : F}
+:
+  Converts FUnit.conversion
+    ((eq0 a).getState state)
+    ((eq0 a).getResult state.numAlloc state.σ)
+    ()
+:= by
+  constructor <;> simp at *
+
+lemma constraints
+  {state : ClapMState p}
+  {a}
+  {a_val : ZMod p}
+  (h_a : Converts F.conversion state a a_val)
+:
+  ((eq0 a).runAndEval state.numAlloc state.varStore state.σ).2.constraints ↔
+  (a_val = 0)
+:= by
+  simp
+  have := h_a.value_eq
+  simp at this
+  simp [this]
+
+lemma convertsM
+  [p.AtLeastTwo]
+  {state}
+  {a : F}
+  {a_val : ZMod p}
+  (h_a : Converts F.conversion state a a_val)
+:
+  ConvertsM FUnit.conversion (eq0 a)
+    state
+    ()
+    (a_val = 0)
+where
+  result := converts
+  wellFormed := wellFormed h_a
+  constraints := constraints h_a
+
+end eq0
+
+end Clap.Lang
