Clap/eDSLState/Convert/Specialised.lean
@@ -1,0 +1,365 @@
+import Clap.eDSLState.Convert.Base
+
+import Clap.Lang.Wheels
+import Clap.Lang.F.Tactics
+
+namespace Clap.Lang
+
+variable {p : ℕ}
+
+abbrev F := ExprRef
+abbrev FB := F
+abbrev FArray (k) := Vector FB k -- TODO FB_Vector?
+abbrev FList := List FB
+
+section Converts
+
+namespace F
+
+abbrev conversion : Conversion p F where
+  IdealT := ZMod p
+  toExprs x := [x]
+  conversion x := [x]
+
+end F
+
+
+namespace FB
+
+abbrev conversion : Conversion p FB where
+  IdealT := Bool
+  toExprs x := [x]
+  conversion x := [if x then 1 else 0]
+
+end FB
+
+
+namespace FUnit
+
+abbrev conversion : Conversion p Unit where
+  IdealT := Unit
+  toExprs _ := []
+  conversion _ := []
+
+end FUnit
+
+
+namespace FArray
+
+abbrev conversion {k} : Conversion p (FArray k) where
+  IdealT := Vector Bool k
+  toExprs x := x.toList
+  conversion x := (x.map fun x ↦ if x then 1 else 0).toList
+
+end FArray
+
+
+namespace FList
+
+abbrev conversion : Conversion p FList where
+  IdealT := List Bool
+  toExprs x := x
+  conversion x := x.map fun x ↦ if x then 1 else 0
+
+end FList
+
+end Converts
+
+
+section ConvertsLemmas
+
+namespace F
+
+lemma converts_of_FB_converts
+  {state : ClapMState p}
+  {expr : FB}
+  {b : Bool}
+  (h : Converts FB.conversion state expr b)
+:
+  Converts F.conversion state expr (if b then (1 : ZMod p) else (0 : ZMod p))
+:= converts_cast
+  (conversion1 := FB.conversion)
+  (conversion2 := F.conversion)
+  (y := expr)
+  (val2 := if b then (1 : ZMod p) else (0 : ZMod p))
+  h (by rfl) (by rfl)
+
+end F
+
+namespace FB
+
+lemma converts_of_F_converts
+  [p.AtLeastTwo]
+  {state : ClapMState p}
+  {expr : F}
+  {val}
+  (h : Converts F.conversion state expr val)
+  (h_val : val.val < 2)
+:
+  Converts FB.conversion state (expr : FB) (val == 1)
+:= by
+  apply converts_cast h
+  . rfl
+  . unfold F.conversion conversion
+    simp
+    split
+    . trivial
+    next h_neq =>
+      rewrite [←ZMod.val_eq_zero]
+      rewrite [←ZMod.val_eq_one] at h_neq
+      grind
+      exact Nat.AtLeastTwo.one_lt
+
+lemma convertsM_of_F_convertsM
+  [p.AtLeastTwo]
+  {action : ClapM p F}
+  {state : ClapMState p}
+  {val : ZMod p}
+  {constraints}
+  (h : ConvertsM F.conversion action state val constraints)
+  (h_val : val.val < 2)
+:
+  ConvertsM FB.conversion action state (val == 1) constraints
+:= by
+  constructor
+  . exact converts_of_F_converts h.result h_val
+  . exact h.wellFormed
+  . exact h.constraints
+
+end FB
+
+
+namespace FUnit
+
+lemma converts
+  {state : ClapMState p}
+  {exprs}
+  {val}
+:
+  Converts FUnit.conversion state exprs val
+:= by
+  grind [Converts]
+
+end FUnit
+
+
+namespace FArray
+
+@[simp]
+lemma converts_empty
+  {state : ClapMState p}
+:
+  Converts conversion state #v[] #v[]
+:= by
+  constructor
+  . grind
+  · grind
+  · grind
+  · grind
+
+lemma converts_iff_FB_converts
+  {k}
+  {state : ClapMState p}
+  {exprs : FArray k}
+  {val : Vector Bool k}
+:
+  Converts conversion state exprs val ↔
+  (∀ i : Fin k, Converts FB.conversion state exprs[i] val[i])
+:= by
+  constructor
+  . intro h ⟨i, h_i⟩
+    constructor
+    . intro ⟨ib, h_ib⟩
+      simp
+      convert h.varSet_wf ⟨i, by grind⟩
+      simp [conversion]
+    . intro ⟨ib, h_ib⟩
+      simp
+      convert h.expr_wf ⟨i, by grind⟩
+      simp [conversion]
+    . intro ⟨ib, h_ib⟩
+      simp
+      convert h.value_eq ⟨i, by grind⟩
+      . simp [conversion]
+      . simp [conversion]
+    . rfl
+  . intro h
+    constructor
+    . intro ⟨i, h_i⟩
+      convert (h ⟨i, by grind⟩).varSet_wf
+      simp [conversion]
+    . intro ⟨i, h_i⟩
+      convert (h ⟨i, by grind⟩).expr_wf
+      simp [conversion]
+    . intro ⟨i, h_i⟩
+      convert (h ⟨i, by grind⟩).value_eq
+      simp [conversion]
+    . grind
+
+lemma converts_push
+  {k}
+  {state : ClapMState p}
+  {exprs : Vector FB k}
+  {expr : FB}
+  {vals : Vector Bool k}
+  {val : Bool}
+  (h_exprs : Converts conversion state exprs vals)
+  (h_expr : Converts FB.conversion state expr val)
+:
+  Converts conversion state (exprs.push expr) (vals.push val)
+:= by
+  rewrite [converts_iff_FB_converts] at h_exprs ⊢
+  intro ⟨i, h_i⟩
+  by_cases i = k
+  . convert h_expr
+    . grind
+    . grind
+  . convert (h_exprs ⟨i, by grind⟩) using 1
+    . grind
+    . grind
+
+lemma convertsM_of_convertsM_toList
+  {k}
+  {action : ClapM p (Vector FB k)}
+  {state}
+  {val : Vector Bool k}
+  {constraints}
+  (h : ConvertsM FList.conversion (Vector.toList <$> action) state val.toList constraints)
+:
+  ConvertsM conversion action state val constraints
+:= by
+  constructor
+  . obtain ⟨⟨_, _, _, _⟩, _, _⟩ := h
+    constructor <;> simp at *
+    . assumption
+    . assumption
+    . assumption
+  . grind [h.wellFormed]
+  . grind [h.constraints, ClapM.runAndEval]
+
+lemma converts_vector_cast
+  {k1 k2}
+  {state : ClapMState p}
+  {exprs : FArray k1}
+  {val : Vector Bool k1}
+  (h : Converts conversion state exprs val)
+  (h_k : k1 = k2)
+:
+  Converts conversion state (exprs.cast h_k) (val.cast h_k)
+:= by
+  rewrite [converts_iff_FB_converts] at ⊢ h
+  intro ⟨i, h_i⟩
+  exact h ⟨i, by grind⟩
+
+lemma converts_pop
+  {k}
+  {state : ClapMState p}
+  {exprs : FArray k}
+  {val : Vector Bool k}
+  (h : Converts conversion state exprs val)
+:
+  Converts conversion state (exprs.pop) (val.pop)
+:= by
+  rewrite [converts_iff_FB_converts] at ⊢ h
+  intro ⟨i, h_i⟩
+  convert (h ⟨i, by grind⟩) using 1
+  . grind
+  . grind
+
+lemma converts_getElem
+  {k i}
+  {state : ClapMState p}
+  {exprs : FArray k}
+  {vals : Vector Bool k}
+  (h : Converts conversion state exprs vals)
+  (h_i : i < k)
+:
+  Converts FB.conversion state exprs[i] vals[i]
+:= (converts_iff_FB_converts.mp h) ⟨i, h_i⟩
+
+end FArray
+
+
+namespace FList
+
+@[simp]
+lemma converts_empty
+  {state : ClapMState p}
+: Converts conversion state [] [] := by
+  constructor
+  . simp
+  · simp
+  · grind
+  · grind
+
+lemma converts_append
+  {state : ClapMState p}
+  {exprs1 exprs2 : List FB}
+  {vals1 vals2 : List Bool}
+  (h_exprs1 : Converts FList.conversion state exprs1 vals1)
+  (h_exprs2 : Converts FList.conversion state exprs2 vals2)
+:
+  Converts FList.conversion state (exprs1 ++ exprs2) (vals1 ++ vals2)
+:= by
+  obtain ⟨exprs1_length, exprs1_varSet, exprs1_wellFormed, exprs1_result⟩ := h_exprs1
+  obtain ⟨exprs2_lengh, exprs2_varSet, exprs2_wellFormed, exprs2_result⟩ := h_exprs2
+  simp at *
+  constructor
+  . intro i
+    simp [List.getElem_append]
+    split
+    . exact exprs1_varSet ⟨i.val, by grind⟩
+    . exact exprs2_varSet ⟨_, by grind⟩
+  . intro i
+    simp [List.getElem_append]
+    split
+    . exact exprs1_wellFormed ⟨i.val, by grind⟩
+    . exact exprs2_wellFormed ⟨_, by grind⟩
+  . intro i
+    simp [List.getElem_append, exprs1_length]
+    split
+    . exact exprs1_result ⟨i.val, by grind⟩
+    . exact exprs2_result ⟨_, by grind⟩
+  . grind
+
+lemma converts_of_converts_FB
+  {state : ClapMState p}
+  {exprs}
+  {vals}
+  (h_length : exprs.length = vals.length)
+  (h_converts : ∀ i : Fin exprs.length, Converts FB.conversion state exprs[i] vals[i])
+:
+  Converts FList.conversion state exprs vals
+:= by
+  constructor
+  . intro i
+    have := (h_converts i).varSet_wf
+    simp at this
+    assumption
+  . intro i
+    have := (h_converts i).expr_wf
+    simp at this
+    assumption
+  . intro i
+    have := (h_converts i).value_eq
+    simp at this
+    simp [this]
+  . grind
+
+lemma converts_singleton_of_converts_FB
+  {state : ClapMState p}
+  {expr}
+  {val}
+  (h_converts : Converts FB.conversion state expr val)
+:
+  Converts FList.conversion state [expr] [val]
+:= by
+  apply converts_of_converts_FB
+  . simpa
+  . simp
+
+end FList
+
+end ConvertsLemmas
+
+end Clap.Lang
